src/Narcissus/ComplementaryFormats/ComplementaryFormat.v
@@ -1,0 +1,62 @@
+Require Import
+        Fiat.Computation
+        Fiat.Common.DecideableEnsembles
+        Fiat.Narcissus.Common.Specs
+        Fiat.Narcissus.Common.Notations.
+
+Section ComplementaryFormats.
+
+  Variable A : Type.  (* Source Type, i.e. in-memory data *)
+  Variable NA : Type. (* Not Source Type used to generate invalid target data *)
+  Variable B : Type.  (* Target Type, usually ByteStrings *)
+  Context {monoid_B : Monoid B}. (* Target type needs to be a monoid. *)
+
+  Variable store : Cache. (* Store Type *)
+  Variable Nstore : Cache. (* Not Store Type *)
+
+  Variable Format : @FormatM A B store. (* The source format *)
+  Variable NFormat : @FormatM NA B Nstore. (* The format of invalid bytestrings *)
+  Variable NA_OK : NA -> Prop. (* Not source data property that ensures it will
+                                generate invalid bytestrings *)
+  
+  Notation "a ∋ b" := (@computes_to _ a b) (at level 90).
+  Notation "a ∌ b" := (~ @computes_to _ a b) (at level 90).
+
+  (* To start, we define the set of invalid bytestrings for a format. *)
+  Definition ComplementaryFormat
+             (decode_inv : @CacheDecode store -> Prop) :=
+    forall na b ns ns',
+      NFormat na ns ∋ (b, ns') (* If a bytestring is in the invalid format *)
+      -> NA_OK na              (* and the data was not okay *)
+      -> forall a s s' s'',
+        decode_inv s'' (* The binary string could not have been produced by *)
+        -> Equiv s s'' (* an encoder that was started in a state equivalent to a *)
+        -> Format a s ∌ (b, s')  (* valid decoder state (this should be the empty state) *).
+        
+  (* Now, we want to be able to derive conditions on the invalid format that ensure
+     it is complementary. *)
+  Definition CorrectDecoderComplement
+    : forall (predicate : A -> Prop)
+             (predicate_OK :
+                forall a s b s',
+                  Format a s ∋ (b, s')
+                  -> predicate a)
+             (rest_predicate : A -> B -> Prop := fun _ _ => True)
+             (decode : @DecodeM A B store)
+             (decode_inv : CacheDecode -> Prop),
+      CorrectDecoder _ predicate rest_predicate Format decode decode_inv
+      -> (forall na b ns ns',
+             NA_OK na
+             -> NFormat na ns ∋ (b, ns')
+             -> forall s b',
+               decode_inv s
+               -> decode (mappend b b') s = None)
+      -> ComplementaryFormat decode_inv.
+  Proof.
+    unfold ComplementaryFormat, CorrectDecoder; intros.
+    intro.
+    eapply H0 in H1; eauto.
+    exact (@CorrectDecoderNone _ _ _ _ _ _ _ _ _ H _ mempty _ H3 H1 _ _ _ H4 (predicate_OK _ _ _ _ H5) I H5).
+  Qed.
+
+End ComplementaryFormats.
